examples/miniML/compiler/CompileScript.sml
@@ -32,6 +32,15 @@ val _ = Defn.save_defn find_index_defn;
 
 (*open MiniML*)
 
+(* TODO: elsewhere? *)
+ val map_result_defn = Hol_defn "map_result" `
+
+(map_result f (Rval v) = Rval (f v))
+/\
+(map_result f (Rerr e) = Rerr e)`;
+
+val _ = Defn.save_defn map_result_defn;
+
 (* observable values *)
 
 val _ = Hol_datatype `
@@ -168,68 +177,62 @@ val _ = Defn.save_defn CevalPrim2_defn;
 
 val _ = Defn.save_defn Cpmatch_defn;
 
-val _ = Hol_datatype `
-(*  'a *) Cresult =
-    CRval of 'a
-  | CRerr of error`;
-
-
 val _ = Hol_reln `
 (! env error.
 T
 ==>
-Cevaluate env (CRaise error) (CRerr error))
+Cevaluate env (CRaise error) (Rerr (Rraise error)))
 
 /\
 (! env n v. ($=)
 (FAPPLY  env  n) v
 ==>
-Cevaluate env (CVar n) (CRval v))
+Cevaluate env (CVar n) (Rval v))
 
 /\
 (! env l.
 T
 ==>
-Cevaluate env (CVal (CLit l)) (CRval (CLit l)))
+Cevaluate env (CVal (CLit l)) (Rval (CLit l)))
 
 /\
 (! env n es vs.
-Cevaluate_list env es (CRval vs)
+Cevaluate_list env es (Rval vs)
 ==>
-Cevaluate env (CCon n es) (CRval (CConv n vs)))
+Cevaluate env (CCon n es) (Rval (CConv n vs)))
 /\
 (! env n es err.
-Cevaluate_list env es (CRerr err)
+Cevaluate_list env es (Rerr err)
 ==>
-Cevaluate env (CCon n es) (CRerr err))
+Cevaluate env (CCon n es) (Rerr err))
 
 /\
 (! env e n m vs.
-Cevaluate env e (CRval (CConv m vs))
+Cevaluate env e (Rval (CConv m vs))
 ==>
-Cevaluate env (CTagEq e n) (CRval (CLit (Bool ( ($=)n m)))))
+Cevaluate env (CTagEq e n) (Rval (CLit (Bool ( ($=)n m)))))
 /\
 (! env e n err.
-Cevaluate env e (CRerr err)
+Cevaluate env e (Rerr err)
 ==>
-Cevaluate env (CTagEq e n) (CRerr err))
+Cevaluate env (CTagEq e n) (Rerr err))
 
 /\
 (! env e n m vs.
-Cevaluate env e (CRval (CConv m vs))
+Cevaluate env e (Rval (CConv m vs))
 ==>
-Cevaluate env (CProj e n) (CRval (EL  n  vs)))
+Cevaluate env (CProj e n) (Rval (EL  n  vs)))
 /\
 (! env e n err.
-Cevaluate env e (CRerr err)
+Cevaluate env e (Rerr err)
 ==>
-Cevaluate env (CProj e n) (CRerr err))
+Cevaluate env (CProj e n) (Rerr err))
 
 /\
 (! env n.
 T
 ==>
-Cevaluate env (CMat n []) (CRerr Bind_error))
+Cevaluate env (CMat n []) (Rerr (Rraise Bind_error)))
 /\
 (! env n p e pes env' r. ($/\) (($=)
 (Cpmatch env p (FAPPLY  env  n)) (SOME env'))
@@ -250,7 +253,7 @@ Cevaluate env b r
 Cevaluate env (CLet [] [] b) r)
 /\
 (! env n ns e es b v r. ($/\)
-(Cevaluate env e (CRval v))
+(Cevaluate env e (Rval v))
 (Cevaluate (FUPDATE  env ( n, v)) (CLet ns es b) r)
 ==>
 Cevaluate env (CLet (CONS n ns) (CONS e es) b) r)
@@ -281,27 +284,27 @@ Cevaluate env (CLetfun T ns defs b) r)
 (! env ns b.
 T
 ==>
-Cevaluate env (CFun ns b) (CRval (CClosure (fmap_to_alist env) ns b)))
+Cevaluate env (CFun ns b) (Rval (CClosure (fmap_to_alist env) ns b)))
 
 /\
 (! env e es env' ns b vs r. ($/\)
-(Cevaluate env e (CRval (CClosure env' ns b))) (($/\)
-(Cevaluate_list env es (CRval vs))
+(Cevaluate env e (Rval (CClosure env' ns b))) (($/\)
+(Cevaluate_list env es (Rval vs))
 (Cevaluate (FOLDL2  (\ en n v . FUPDATE  en ( n, v)) 
              (alist_to_fmap env')  ns  vs) b r))
 ==>
 Cevaluate env (CCall e es) r)
 /\
 (! env e es env' ns b err. ($/\)
-(Cevaluate env e (CRval (CClosure env' ns b)))
-(Cevaluate_list env es (CRerr err))
+(Cevaluate env e (Rval (CClosure env' ns b)))
+(Cevaluate_list env es (Rerr err))
 ==>
-Cevaluate env (CCall e es) (CRerr err))
+Cevaluate env (CCall e es) (Rerr err))
 
 /\
 (! env e es env' ns' defs n i ns b vs r. ($/\)
-(Cevaluate env e (CRval (CRecClos env' ns' defs n))) (($/\)
-(Cevaluate_list env es (CRval vs)) (($/\) (($=)
+(Cevaluate env e (Rval (CRecClos env' ns' defs n))) (($/\)
+(Cevaluate_list env es (Rval vs)) (($/\) (($=)
 (find_index n ns' 0) (SOME i)) (($/\) (($=)
 (EL  i  defs) (ns,b))
 (Cevaluate
@@ -317,111 +320,111 @@ Cevaluate env (CCall e es) (CRerr err))
 Cevaluate env (CCall e es) r)
 /\
 (! env e es env' ns' defs n err. ($/\)
-(Cevaluate env e (CRval (CRecClos env' ns' defs n)))
-(Cevaluate_list env es (CRerr err))
+(Cevaluate env e (Rval (CRecClos env' ns' defs n)))
+(Cevaluate_list env es (Rerr err))
 ==>
-Cevaluate env (CCall e es) (CRerr err))
+Cevaluate env (CCall e es) (Rerr err))
 
 /\
 (! env e es err.
-Cevaluate env e (CRerr err)
+Cevaluate env e (Rerr err)
 ==>
-Cevaluate env (CCall e es) (CRerr err))
+Cevaluate env (CCall e es) (Rerr err))
 
 /\
 (! env p2 e1 e2 v1 v2 e3 r. ($/\)
-(Cevaluate_list env [e1;e2] (CRval [v1;v2])) (($/\) (($=)
+(Cevaluate_list env [e1;e2] (Rval [v1;v2])) (($/\) (($=)
 (CevalPrim2 p2 v1 v2) e3)
 (Cevaluate env e3 r))
 ==>
 Cevaluate env (CPrim2 p2 e1 e2) r)
 /\
 (! env p2 e1 e2 err.
-Cevaluate_list env [e1;e2] (CRerr err)
+Cevaluate_list env [e1;e2] (Rerr err)
 ==>
-Cevaluate env (CPrim2 p2 e1 e2) (CRerr err))
+Cevaluate env (CPrim2 p2 e1 e2) (Rerr err))
 
 /\
 (! env es v1 v2 e3 r. ($/\)
-(Cevaluate_list env es (CRval [v1;v2])) (($/\) (($=)
+(Cevaluate_list env es (Rval [v1;v2])) (($/\) (($=)
 (doPrim2 F Bool int_le v1 v2) e3)
 (Cevaluate env e3 r))
 ==>
 Cevaluate env (CLprim CLeq es) r)
 /\
 (! env es err.
-Cevaluate_list env es (CRerr err)
+Cevaluate_list env es (Rerr err)
 ==>
-Cevaluate env (CLprim CLeq es) (CRerr err))
+Cevaluate env (CLprim CLeq es) (Rerr err))
 
 /\
 (! env e1 e2 e3 b1 r. ($/\)
-(Cevaluate env e1 (CRval (CLit (Bool b1))))
+(Cevaluate env e1 (Rval (CLit (Bool b1))))
 (Cevaluate env (if b1 then e2 else e3) r)
 ==>
 Cevaluate env (CLprim CIf [e1;e2;e3]) r)
 /\
 (! env e1 e2 e3 err.
-Cevaluate env e1 (CRerr err)
+Cevaluate env e1 (Rerr err)
 ==>
-Cevaluate env (CLprim CIf [e1;e2;e3]) (CRerr err))
+Cevaluate env (CLprim CIf [e1;e2;e3]) (Rerr err))
 
 /\
 (! env e1 e2.
-Cevaluate env e1 (CRval (CLit (Bool F)))
+Cevaluate env e1 (Rval (CLit (Bool F)))
 ==>
-Cevaluate env (CLprim CAnd [e1;e2]) (CRval (CLit (Bool F))))
+Cevaluate env (CLprim CAnd [e1;e2]) (Rval (CLit (Bool F))))
 /\
 (! env e1 e2 r. ($/\)
-(Cevaluate env e1 (CRval (CLit (Bool T))))
+(Cevaluate env e1 (Rval (CLit (Bool T))))
 (Cevaluate env e2 r)
 ==>
 Cevaluate env (CLprim CAnd [e1;e2]) r)
 /\
 (! env e1 e2 err.
-Cevaluate env e1 (CRerr err)
+Cevaluate env e1 (Rerr err)
 ==>
-Cevaluate env (CLprim CAnd [e1;e2]) (CRerr err))
+Cevaluate env (CLprim CAnd [e1;e2]) (Rerr err))
 
 /\
 (! env e1 e2.
-Cevaluate env e1 (CRval (CLit (Bool T)))
+Cevaluate env e1 (Rval (CLit (Bool T)))
 ==>
-Cevaluate env (CLprim COr [e1;e2]) (CRval (CLit (Bool T))))
+Cevaluate env (CLprim COr [e1;e2]) (Rval (CLit (Bool T))))
 /\
 (! env e1 e2 r. ($/\)
-(Cevaluate env e1 (CRval (CLit (Bool F))))
+(Cevaluate env e1 (Rval (CLit (Bool F))))
 (Cevaluate env e2 r)
 ==>
 Cevaluate env (CLprim COr [e1;e2]) r)
 /\
 (! env e1 e2 err.
-Cevaluate env e1 (CRerr err)
+Cevaluate env e1 (Rerr err)
 ==>
-Cevaluate env (CLprim COr [e1;e2]) (CRerr err))
+Cevaluate env (CLprim COr [e1;e2]) (Rerr err))
 
 /\
 (! env.
 T
 ==>
-Cevaluate_list env [] (CRval []))
+Cevaluate_list env [] (Rval []))
 /\
 (! env e es v vs. ($/\)
-(Cevaluate env e (CRval v))
-(Cevaluate_list env es (CRval vs))
+(Cevaluate env e (Rval v))
+(Cevaluate_list env es (Rval vs))
 ==>
-Cevaluate_list env (CONS e es) (CRval (CONS v vs)))
+Cevaluate_list env (CONS e es) (Rval (CONS v vs)))
 /\
 (! env e es err.
-Cevaluate env e (CRerr err)
+Cevaluate env e (Rerr err)
 ==>
-Cevaluate_list env (CONS e es) (CRerr err))
+Cevaluate_list env (CONS e es) (Rerr err))
 /\
 (! env e es v err. ($/\)
-(Cevaluate env e (CRval v))
-(Cevaluate_list env es (CRerr err))
+(Cevaluate env e (Rval v))
+(Cevaluate_list env es (Rerr err))
 ==>
-Cevaluate_list env (CONS e es) (CRerr err))`;
+Cevaluate_list env (CONS e es) (Rerr err))`;
 
 val _ = Define `
  (least_not_in s = $LEAST (\ n . ~  ( ($IN)n s)))`;
